HoareLogic/ConcurrentSemantics.v
@@ -4,15 +4,20 @@ Require Import Logic.HoareLogic.ImperativeLanguage.
 Require Import Logic.HoareLogic.ProgramState.
 Require Import Logic.HoareLogic.BigStepSemantics.
 
-Class ThreadLocalBigStepSemantics (P: ProgrammingLanguage) (state: Type) (guard: Type): Type :=
-  guarded_BSS: guard -> BigStepSemantics P state.
+Definition DecorateProgram (P: ProgrammingLanguage) (hint: cmd -> Type): ProgrammingLanguage :=
+  Build_ProgrammingLanguage (sigT hint).
+
+Class ThreadLocalBigStepSemantics (P: ProgrammingLanguage) (state: Type) (guard: Type): Type := {
+  hint: guard -> cmd -> Type;
+  guarded_BSS: forall g: guard, BigStepSemantics (DecorateProgram P (hint g)) state
+}.
 
 Definition tl_access
            {P: ProgrammingLanguage}
            {state: Type}
            {guard: Type}
            {TLBSS: ThreadLocalBigStepSemantics P state guard}:
-  guard -> state -> cmd -> MetaState state -> Prop :=
+  forall (g: guard), state -> sigT (hint g) -> MetaState state -> Prop :=
   fun g => @access _ _ (guarded_BSS g).
 
 Definition lift_tl_access
@@ -20,11 +25,5 @@ Definition lift_tl_access
            {state: Type}
            {guard: Type}
            {TLBSS: ThreadLocalBigStepSemantics P state guard}:
-  guard -> MetaState state -> cmd -> MetaState state -> Prop :=
+  forall g: guard, MetaState state -> sigT (hint g) -> MetaState state -> Prop :=
   fun g => @lift_access _ _ (guarded_BSS g).
-
-(*
-Class NormalBigStepSemantics (P: ProgrammingLanguage) (state: Type) (BSS: BigStepSemantics P state): Type := {
-  access_defined: forall s c, exists ms, access s c ms
-}.
-*)
